src/Std/Data/DHashMap/Lemmas.lean
@@ -2889,6 +2889,11 @@ end DHashMap
 namespace DHashMap
 
 @[simp, grind =]
+theorem ofArray_eq_ofList (a : Array ((a : α) × (β a))) :
+    ofArray a = ofList a.toList :=
+  ext <| congrArg Subtype.val <| congrArg Subtype.val (Raw₀.insertMany_array_eq_insertMany_toList (α := α) _ a)
+
+@[simp, grind =]
 theorem ofList_nil :
     ofList ([] : List ((a : α) × (β a))) = ∅ :=
   ext <| congrArg Subtype.val (Raw₀.insertMany_emptyWithCapacity_list_nil (α := α))
@@ -3038,6 +3043,11 @@ namespace Const
 variable {β : Type v}
 
 @[simp, grind =]
+theorem ofArray_eq_ofList (a : Array (α × β)) :
+    ofArray a = ofList a.toList :=
+  ext <| congrArg Subtype.val <| congrArg Subtype.val (Raw₀.Const.insertMany_array_eq_insertMany_toList (α := α) _ a)
+
+@[simp, grind =]
 theorem ofList_nil :
     ofList ([] : List (α × β)) = ∅ :=
   ext <| congrArg Subtype.val (Raw₀.Const.insertMany_emptyWithCapacity_list_nil (α:= α))
@@ -3181,6 +3191,11 @@ theorem isEmpty_ofList [EquivBEq α] [LawfulHashable α]
     {l : List (α × β)} :
     (ofList l).isEmpty = l.isEmpty :=
   Raw₀.Const.isEmpty_insertMany_emptyWithCapacity_list
+
+@[simp, grind =]
+theorem unitOfArray_eq_unitOfList (a : Array α) :
+    unitOfArray a = unitOfList a.toList :=
+  ext <| congrArg Subtype.val <| congrArg Subtype.val (Raw₀.Const.insertManyIfNewUnit_array_eq_insertManyIfNewUnit_toList (α := α) _ a)
 
 @[simp]
 theorem unitOfList_nil :
