src/Std/Data/HashMap/RawLemmas.lean
@@ -2157,6 +2157,12 @@ theorem size_ofList_le [EquivBEq α] [LawfulHashable α]
 grind_pattern size_ofList_le => (ofList l).size
 
 @[simp, grind =]
+theorem ofArray_eq_ofList (a : Array (α × β)) :
+    ofArray a = ofList a.toList := by
+  apply ext
+  apply DHashMap.Raw.Const.ofArray_eq_ofList
+
+@[simp, grind =]
 theorem isEmpty_ofList [EquivBEq α] [LawfulHashable α]
     {l : List (α × β)} :
     (ofList l).isEmpty = l.isEmpty :=
@@ -2243,6 +2249,12 @@ theorem size_unitOfList_le [EquivBEq α] [LawfulHashable α]
     {l : List α} :
     (unitOfList l).size ≤ l.length :=
   DHashMap.Raw.Const.size_unitOfList_le
+
+@[simp, grind =]
+theorem unitOfArray_eq_unitOfList (a : Array α) :
+    unitOfArray a = unitOfList a.toList := by
+  apply ext
+  apply DHashMap.Raw.Const.unitOfArray_eq_unitOfList
 
 @[simp]
 theorem isEmpty_unitOfList [EquivBEq α] [LawfulHashable α]
